examples/ghc/lib/CoreTidy.v
@@ -1,0 +1,210 @@
+(* Default settings (from HsToCoq.Coq.Preamble) *)
+
+Generalizable All Variables.
+
+Unset Implicit Arguments.
+Set Maximal Implicit Insertion.
+Unset Strict Implicit.
+Unset Printing Implicit Defensive.
+
+Require Coq.Program.Tactics.
+Require Coq.Program.Wf.
+
+(* Converted imports: *)
+
+Require CoreArity.
+Require CoreSyn.
+Require Data.Traversable.
+Require GHC.Base.
+Require GHC.List.
+Require GHC.Prim.
+Require Id.
+Require IdInfo.
+Require Maybes.
+Require Name.
+Require OccName.
+Require SrcLoc.
+Require UniqFM.
+Require Var.
+Require VarEnv.
+
+(* No type declarations to convert. *)
+(* Converted value declarations: *)
+
+Definition op_zeZC__ {a} {b} : a -> (a -> b) -> b :=
+  fun m k => GHC.Prim.seq m (k m).
+
+Notation "'_=:_'" := (op_zeZC__).
+
+Infix "=:" := (_=:_) (at level 99).
+
+Definition tidyIdBndr
+   : VarEnv.TidyEnv -> Var.Id -> (VarEnv.TidyEnv * Var.Id)%type :=
+  fun arg_0__ arg_1__ =>
+    match arg_0__, arg_1__ with
+    | (pair tidy_env var_env as env), id =>
+        let 'pair tidy_env' occ' := OccName.tidyOccName tidy_env (Name.getOccName id) in
+        let old_info := (@Var.idInfo tt id) in
+        let old_unf := IdInfo.unfoldingInfo old_info in
+        let new_unf := CoreSyn.noUnfolding in
+        let new_info :=
+          IdInfo.setOneShotInfo (IdInfo.setOccInfo IdInfo.vanillaIdInfo (IdInfo.occInfo
+                                                    old_info)) (IdInfo.oneShotInfo old_info) in
+        let name' := Name.mkInternalName (Id.idUnique id) occ' SrcLoc.noSrcSpan in
+        let ty' := tt in
+        let id' := Id.mkLocalIdWithInfo name' ty' new_info in
+        let var_env' := VarEnv.extendVarEnv var_env id id' in
+        pair (pair tidy_env' var_env') id'
+    end.
+
+Definition tidyBndr
+   : VarEnv.TidyEnv -> Var.Var -> (VarEnv.TidyEnv * Var.Var)%type :=
+  fun env var => tidyIdBndr env var.
+
+Definition tidyBndrs
+   : VarEnv.TidyEnv -> list Var.Var -> (VarEnv.TidyEnv * list Var.Var)%type :=
+  fun env vars => Data.Traversable.mapAccumL tidyBndr env vars.
+
+Definition tidyLetBndr
+   : VarEnv.TidyEnv ->
+     VarEnv.TidyEnv ->
+     (Var.Id * CoreSyn.CoreExpr)%type -> (VarEnv.TidyEnv * Var.Var)%type :=
+  fun arg_0__ arg_1__ arg_2__ =>
+    match arg_0__, arg_1__, arg_2__ with
+    | rec_tidy_env, (pair tidy_env var_env as env), pair id rhs =>
+        let 'pair tidy_env' occ' := OccName.tidyOccName tidy_env (Name.getOccName id) in
+        let old_info := (@Var.idInfo tt id) in
+        let old_unf := IdInfo.unfoldingInfo old_info in
+        let new_unf := CoreSyn.noUnfolding in
+        let new_info :=
+          IdInfo.setInlinePragInfo (IdInfo.setArityInfo (IdInfo.setOccInfo
+                                                         IdInfo.vanillaIdInfo (IdInfo.occInfo old_info))
+                                                        (CoreArity.exprArity rhs)) (IdInfo.inlinePragInfo old_info) in
+        let details := Var.idDetails id in
+        let name' := Name.mkInternalName (Id.idUnique id) occ' SrcLoc.noSrcSpan in
+        let ty' := tt in
+        let id' := Var.mkLocalVar details name' ty' new_info in
+        let var_env' := VarEnv.extendVarEnv var_env id id' in
+        pair (pair tidy_env' var_env') id'
+    end.
+
+Definition tidyNameOcc : VarEnv.TidyEnv -> Name.Name -> Name.Name :=
+  fun arg_0__ arg_1__ =>
+    match arg_0__, arg_1__ with
+    | pair _ var_env, n =>
+        match UniqFM.lookupUFM var_env n with
+        | None => n
+        | Some v => Id.idName v
+        end
+    end.
+
+Definition tidyVarOcc : VarEnv.TidyEnv -> Var.Var -> Var.Var :=
+  fun arg_0__ arg_1__ =>
+    match arg_0__, arg_1__ with
+    | pair _ var_env, v => Maybes.orElse (VarEnv.lookupVarEnv var_env v) v
+    end.
+
+Definition tidyTickish
+   : VarEnv.TidyEnv -> CoreSyn.Tickish Var.Id -> CoreSyn.Tickish Var.Id :=
+  fun arg_0__ arg_1__ =>
+    match arg_0__, arg_1__ with
+    | env, CoreSyn.Breakpoint ix ids =>
+        CoreSyn.Breakpoint ix (GHC.Base.map (tidyVarOcc env) ids)
+    | _, other_tickish => other_tickish
+    end.
+
+Definition tidyBind
+   : VarEnv.TidyEnv ->
+     CoreSyn.CoreBind -> (VarEnv.TidyEnv * CoreSyn.CoreBind)%type :=
+  fix tidyExpr arg_0__ arg_1__
+        := match arg_0__, arg_1__ with
+           | env, CoreSyn.Var v => CoreSyn.Var (tidyVarOcc env v)
+           | env, CoreSyn.Type_ ty => CoreSyn.Type_ (tt)
+           | env, CoreSyn.Coercion co => CoreSyn.Coercion (tt)
+           | _, CoreSyn.Lit lit => CoreSyn.Lit lit
+           | env, CoreSyn.App f a => CoreSyn.App (tidyExpr env f) (tidyExpr env a)
+           | env, CoreSyn.Tick t e => CoreSyn.Tick (tidyTickish env t) (tidyExpr env e)
+           | env, CoreSyn.Cast e co => CoreSyn.Cast (tidyExpr env e) (tt)
+           | env, CoreSyn.Let b e =>
+               tidyBind env b =: (fun '(pair env' b') => CoreSyn.Let b' (tidyExpr env' e))
+           | env, CoreSyn.Case e b ty alts =>
+               tidyBndr env b =:
+               (fun '(pair env' b) =>
+                  CoreSyn.Case (tidyExpr env e) b (tt) (GHC.Base.map ((fun env x =>
+                                                                         let 'pair (pair con vs) rhs := x in
+                                                                         let 'pair env' vs := tidyBndrs env vs in
+                                                                         pair (pair con vs) (tidyExpr env' rhs)) env')
+                                                        alts))
+           | env, CoreSyn.Lam b e =>
+               tidyBndr env b =: (fun '(pair env' b) => CoreSyn.Lam b (tidyExpr env' e))
+           end with tidyBind arg_0__ arg_1__
+                      := match arg_0__, arg_1__ with
+                         | env, CoreSyn.NonRec bndr rhs =>
+                             tidyLetBndr env env (pair bndr rhs) =:
+                             (fun '(pair env' bndr') => pair env' (CoreSyn.NonRec bndr' (tidyExpr env' rhs)))
+                         | env, CoreSyn.Rec prs =>
+                             let 'pair env' bndrs' := Data.Traversable.mapAccumL (tidyLetBndr env) env prs in
+                             GHC.Base.map (fun x => tidyExpr env' (snd x)) prs =:
+                             (fun rhss' => pair env' (CoreSyn.Rec (GHC.List.zip bndrs' rhss')))
+                         end for tidyBind.
+
+Definition tidyExpr : VarEnv.TidyEnv -> CoreSyn.CoreExpr -> CoreSyn.CoreExpr :=
+  fix tidyExpr arg_0__ arg_1__
+        := match arg_0__, arg_1__ with
+           | env, CoreSyn.Var v => CoreSyn.Var (tidyVarOcc env v)
+           | env, CoreSyn.Type_ ty => CoreSyn.Type_ (tt)
+           | env, CoreSyn.Coercion co => CoreSyn.Coercion (tt)
+           | _, CoreSyn.Lit lit => CoreSyn.Lit lit
+           | env, CoreSyn.App f a => CoreSyn.App (tidyExpr env f) (tidyExpr env a)
+           | env, CoreSyn.Tick t e => CoreSyn.Tick (tidyTickish env t) (tidyExpr env e)
+           | env, CoreSyn.Cast e co => CoreSyn.Cast (tidyExpr env e) (tt)
+           | env, CoreSyn.Let b e =>
+               tidyBind env b =: (fun '(pair env' b') => CoreSyn.Let b' (tidyExpr env' e))
+           | env, CoreSyn.Case e b ty alts =>
+               tidyBndr env b =:
+               (fun '(pair env' b) =>
+                  CoreSyn.Case (tidyExpr env e) b (tt) (GHC.Base.map ((fun env x =>
+                                                                         let 'pair (pair con vs) rhs := x in
+                                                                         let 'pair env' vs := tidyBndrs env vs in
+                                                                         pair (pair con vs) (tidyExpr env' rhs)) env')
+                                                        alts))
+           | env, CoreSyn.Lam b e =>
+               tidyBndr env b =: (fun '(pair env' b) => CoreSyn.Lam b (tidyExpr env' e))
+           end with tidyBind arg_0__ arg_1__
+                      := match arg_0__, arg_1__ with
+                         | env, CoreSyn.NonRec bndr rhs =>
+                             tidyLetBndr env env (pair bndr rhs) =:
+                             (fun '(pair env' bndr') => pair env' (CoreSyn.NonRec bndr' (tidyExpr env' rhs)))
+                         | env, CoreSyn.Rec prs =>
+                             let 'pair env' bndrs' := Data.Traversable.mapAccumL (tidyLetBndr env) env prs in
+                             GHC.Base.map (fun x => tidyExpr env' (snd x)) prs =:
+                             (fun rhss' => pair env' (CoreSyn.Rec (GHC.List.zip bndrs' rhss')))
+                         end for tidyExpr.
+
+Definition tidyAlt : VarEnv.TidyEnv -> CoreSyn.CoreAlt -> CoreSyn.CoreAlt :=
+  fun arg_0__ arg_1__ =>
+    match arg_0__, arg_1__ with
+    | env, pair (pair con vs) rhs =>
+        tidyBndrs env vs =:
+        (fun '(pair env' vs) => pair (pair con vs) (tidyExpr env' rhs))
+    end.
+
+Module Notations.
+Notation "'_CoreTidy.=:_'" := (op_zeZC__).
+Infix "CoreTidy.=:" := (_=:_) (at level 99).
+End Notations.
+
+(* External variables:
+     None Some list op_zt__ pair snd tt CoreArity.exprArity CoreSyn.App
+     CoreSyn.Breakpoint CoreSyn.Case CoreSyn.Cast CoreSyn.Coercion CoreSyn.CoreAlt
+     CoreSyn.CoreBind CoreSyn.CoreExpr CoreSyn.Lam CoreSyn.Let CoreSyn.Lit
+     CoreSyn.NonRec CoreSyn.Rec CoreSyn.Tick CoreSyn.Tickish CoreSyn.Type_
+     CoreSyn.Var CoreSyn.noUnfolding Data.Traversable.mapAccumL GHC.Base.map
+     GHC.List.zip GHC.Prim.seq Id.idName Id.idUnique Id.mkLocalIdWithInfo
+     IdInfo.inlinePragInfo IdInfo.occInfo IdInfo.oneShotInfo IdInfo.setArityInfo
+     IdInfo.setInlinePragInfo IdInfo.setOccInfo IdInfo.setOneShotInfo
+     IdInfo.unfoldingInfo IdInfo.vanillaIdInfo Maybes.orElse Name.Name
+     Name.getOccName Name.mkInternalName OccName.tidyOccName SrcLoc.noSrcSpan
+     UniqFM.lookupUFM Var.Id Var.Var Var.idDetails Var.idInfo Var.mkLocalVar
+     VarEnv.TidyEnv VarEnv.extendVarEnv VarEnv.lookupVarEnv
+*)
