examples/ghc/deps/CoreArity.mk
@@ -1,1 +1,1 @@
-lib/CoreArity.v: lib/CoreSyn.h2ci
+lib/CoreArity.v: 
