examples/ghc/deps/CoreTidy.mk
@@ -1,0 +1,1 @@
+lib/CoreTidy.v: lib/CoreSyn.h2ci
